\documentclass{article}
\usepackage{amsmath}
\usepackage{amsfonts}
\usepackage{amssymb}
\usepackage{xcolor}
\author{Nick Daiber}
\title{Mathe 09}
\begin{document}
\section*{1}
\subsection*{a}
\subsubsection*{1}
\begin{align*}
    (1+i)^{-1}(1+i)&=1\\
    (a+bi)(1+i)&=1\\
    a+ai+bi-b&=1\\
    (a-b)+(a+b)i&=1\\
    |(a-b)+(a+b)i|&=|1|\\
    (a-b)^2+(a+b)^2&=1\\
    a^2-2ab+b^2+a^2+2ab+b^2&=1\\
    2a^2+2b^2&=1\\
    a^2+b^2&=\frac{1}{2}\\
    \Rightarrow a=\frac{1}{2},b&=-\frac{1}{2}
\end{align*}
\subsubsection*{2}
Zun√§chst $\frac{1}{i}$
\begin{align*}
    \frac{1}{i}\cdot i&=1\\
    (a+bi)i&=1\\
    ai-b&=1\\
    b&=-1\\
    \frac{1}{i}&=-i
\end{align*}
\begin{align*}
    \frac{1}{i}+3\cdot (1+i)^{-1}&=-i + 3 \cdot (0.5-0.5i)\\
    &=1.5-2.5i
\end{align*}
\subsubsection*{3}
\begin{align*}
    \frac{\sqrt{2}}{\sqrt{2}-i}&=a+bi\\
    \sqrt{2}&=(\sqrt{2}-i)(a+bi)\\
    &=\sqrt{2}a+\sqrt{2}bi-ai+b\\
    &=\sqrt{2}a+b+(\sqrt{2}b-a)i\\
    1&=a+\frac{b}{\sqrt{2}}+(b-\frac{a}{\sqrt{2}})i\\
    &=(a+\frac{b}{\sqrt{2}})^2+(b-\frac{a}{\sqrt{2}})^2\\
    &=a^2+\frac{b^2}{2}+\frac{2ab}{\sqrt{2}}+\frac{a^2}{2}+b^2-\frac{2ab}{\sqrt{2}}\\
    &=\frac{3}{2}a^2+ \frac{3}{2}b^2\\
    \frac{2}{3}&=a^2+b^2\\
    &\Rightarrow a=\frac{2}{3}, b=\frac{\sqrt{2}}{3}
\end{align*}
\subsubsection*{4}
\begin{align*}
    \frac{1+i}{1-i}&=a+bi\\
    1+i&=(a+bi)(1-i)\\
    &=a-ai+bi+b\\
    &=(a+b)+(-a+b)i\\
    &\Rightarrow a+b=1,-a+b=1\\
    &\Rightarrow a=0,b=1
\end{align*}
\begin{align*}
    (i)^{201}&=(i^4)^{50}i\\
    &=i^{50}i\\
    &=(i^4)^{10}i^{10}i\\
    &=i^{20}i\\
    &=(i^4)^{5}i\\
    &=i^4i^2\\
    &=-i
\end{align*}
\subsection*{b}
\begin{align*}
    |z+1|&=|z-(1+2i)|\\
    |(a+bi)+1|&=|(a+bi)-(1+2i)|\\
    \sqrt{(a+1)^2+b^2}&=\sqrt{(a-1)^2+(b-2)^2}\\
    (a+1)^2+b^2&=(a-1)^2+(b-2)^2\\
    a^2+2a+1+b^2&=a^2-2a+1+b^2-4b+4\\
    4a&=-4b+4\\
    a+b&=1\\
\end{align*}
\subsection*{c}
\end{document}