\documentclass{article}
\usepackage{amsmath}
\usepackage{amsfonts}
\usepackage{amssymb}
\usepackage{xcolor}
\author{Nick Daiber}
\title{Mathe 07}

\begin{document}
\maketitle
\section*{3}
\subsection*{a}
\begin{tabular}{r|llll}
    i&1&2&3&4\\
    \hline
    $x_i$&0&1&4&5\\
    $y_i$&4&3&3&3\\
\end{tabular}

$L_1 = \frac{(x-1)(x-4)(x-5)}{(-1)(-3)(-5)}$\\
$L_2 = \frac{(x)(x-4)(x-5)}{1\cdot(-3)(-5)}$\\
$L_3 = \frac{(x)(x-1)(x-5)}{4\cdot 3 (-1)}$\\
$L_4 = \frac{(x)(x-1)(x-4)}{5\cdot 4 \cdot 1}$\\
$f(x)= 4L_1(x) + 3L_2(x) + 3L_3(x) + 3L_4(x) = x^3+4x^2+x+4$
\subsection*{b}
\begin{tabular}{rl}
    $x$&$f(x)$\\
    \hline
    0&4\\
    1&3\\
    2&2\\
    3&0\\
    4&3\\
    5&3\\
    6&6
\end{tabular}

$f(x) = (x-c)g(x) = (x-3)g(x)$

\begin{tabular}{r|cccc}
    Koeffizienten&1&4&1&4\\
    $c=3$&&$1\cdot 3=0$&&$1\cdot 3 = 3$\\
    \hline
    $g$:&0&1&0&1
\end{tabular}

$g(x) = x^2+1$
\end{document}